adapt to new Haskell spec (on branch sam1)

src/Program.v
@@ -1,35 +1,7 @@
 Require Import riscv.util.NameWithEq.
 Require Import riscv.Utility.
 Require Import Coq.ZArith.BinInt.
-
-(* t will be instantiated with a signed type, u with an unsigned type.
-   By default, all operations are on signed numbers. *)
-Class Alu(t u: Set) := mkAlu {
-  (* constants *)
-  zero: t;
-  one: t;
-
-  (* arithmetic operations: *)
-  add: t -> t -> t;
-  sub: t -> t -> t;
-  mul: t -> t -> t;
-  div: t -> t -> t;
-  rem: t -> t -> t;
-
-  (* comparison operators: *)
-  signed_less_than: t -> t -> bool;
-  unsigned_less_than: u -> u -> bool;
-  signed_eqb: t -> t -> bool;
-
-  (* logical operations: *)
-  shiftL: t -> Z -> t;
-  signed_shiftR: t -> Z -> t; (* arithmetic shift *)
-  unsigned_shiftR: u -> Z -> u; (* logic shift *)
-
-  xor: t -> t -> t;
-  or: t -> t -> t;
-  and: t -> t -> t;
-}.
+Require Import bbv.Word.
 
 Notation "a <|> b" := (or a b)  (at level 50, left associativity) : alu_scope.
 Notation "a <&> b" := (and a b) (at level 40, left associativity) : alu_scope.
@@ -41,12 +13,9 @@ Notation "a == b" := (signed_eqb a b)               (at level 70, no associativi
 Notation "a < b"  := (signed_less_than a b)         (at level 70, no associativity) : alu_scope.
 Notation "a >= b" := (negb (signed_less_than a b))  (at level 70, no associativity) : alu_scope.
 
-Definition ltu{t u s: Set}{A: Alu t u}{c: Convertible t u}{ic: IntegralConversion s u}
-  (x: t)(y: s): bool := unsigned_less_than (unsigned x) (fromIntegral y: u).
-
 Section Constants.
-  Context {t u: Set}.
-  Context {A: Alu t u}.
+  Context {t: Set}.
+  Context {MW: MachineWidth t}.
 
   Local Open Scope alu_scope.
 
@@ -56,49 +25,24 @@ Section Constants.
 
 End Constants.
 
-Section Shifts.
-
-  Context {t u: Set}.
-  Context {A: Alu t u}.
-  Context {c: Convertible t u}.
-  Context {m: MachineWidth t}.
-  Context {ic0: IntegralConversion Z t}.
-
-  Definition slli(x: t)(shamt6: Z): t :=
-    shiftL x (shiftBits (fromIntegral shamt6: t)).
-
-  Definition srli(x: t)(shamt6: Z): u :=
-    unsigned_shiftR ((unsigned x) : u) (shiftBits (fromIntegral shamt6 : t)).
-
-  Definition srai(x: t)(shamt6: Z): t :=
-    signed_shiftR x (shiftBits (fromIntegral shamt6 : t)).
-
-  Definition sll(x y: t): t := shiftL x (shiftBits y).
-
-  Definition srl(x y: t): u := unsigned_shiftR (unsigned x) (shiftBits y).
-
-  Definition sra(x y: t): t := signed_shiftR x (shiftBits y).
-
-End Shifts.
-
 Section Riscv.
 
   Context {Name: NameWithEq}. (* register name *)
   Notation Register := (@name Name).
 
-  Class RiscvState(M: Type -> Type){t u: Set}{A: Alu t u} := mkRiscvState {
+  Class RiscvState(M: Type -> Type){t: Set}{MW: MachineWidth t} := mkRiscvState {
     getRegister: Register -> M t;
-    setRegister{s: Set}{c: IntegralConversion s t}: Register -> s -> M unit;
+    setRegister: Register -> t -> M unit;
 
-    loadByte: t -> M Int8;
-    loadHalf: t -> M Int16;
-    loadWord: t -> M Int32;
-    loadDouble: t -> M Int64;
+    loadByte: t -> M (word 8);
+    loadHalf: t -> M (word 16);
+    loadWord: t -> M (word 32);
+    loadDouble: t -> M (word 64);
 
-    storeByte: t -> Int8 -> M unit;
-    storeHalf: t -> Int16 -> M unit;
-    storeWord: t -> Int32 -> M unit;
-    storeDouble: t -> Int64 -> M unit;
+    storeByte: t -> word 8 -> M unit;
+    storeHalf: t -> word 16 -> M unit;
+    storeWord: t -> word 32 -> M unit;
+    storeDouble: t -> word 64 -> M unit;
 
     getPC: M t;
     setPC: t -> M unit;
