src/Execute.v
@@ -7,10 +7,6 @@ Require Import riscv.NoVirtualMemory.
 Require Import riscv.Decode.
 Require Import riscv.Program.
 
-Instance icId{t: Set}: IntegralConversion t t := {|
-  fromIntegral := id
-|}.
-
 Local Open Scope Z.
 Local Open Scope alu_scope.
 
@@ -22,67 +18,43 @@ Section Riscv.
 
   Context {B: RiscvBitWidths}.
 
-  Context {t u: Set}.
+  Context {t: Set}.
 
-  Context {A: Alu t u}.
-
-  Context {c: Convertible t u}.
-
-  Context {ic8: IntegralConversion Int8 t}.
-  Context {ic16: IntegralConversion Int16 t}.
-  Context {ic32: IntegralConversion Int32 t}.
-
-  Context {ic8': IntegralConversion t Int8}.
-  Context {ic16': IntegralConversion t Int16}.
-  Context {ic32': IntegralConversion t Int32}.
-
-  Context {ic8u: IntegralConversion Word8 t}.
-  Context {ic16u: IntegralConversion Word16 t}.
-  Context {ic32u: IntegralConversion Word32 t}.
-
-  Context {icZt: IntegralConversion Z t}.
-
-  Context {icZu: IntegralConversion Z u}.
-
-  Context {icut: IntegralConversion u t}.
-  Context {ictu: IntegralConversion t u}.
-
-  Context {m: MachineWidth t}.
+  Context {MW: MachineWidth t}.
 
   Notation "'when' a b" := (if a then b else Return tt) (at level 60, a at level 0, b at level 0).
-
 
   Definition execute{M: Type -> Type}{MM: Monad M}{RVS: RiscvState M}(i: Instruction): M unit :=
     match i with
     (* begin ast *)
     | Lui rd imm20 =>
-        setRegister rd imm20
+        setRegister rd (fromImm imm20)
     | Auipc rd oimm20 =>
         pc <- getPC;
-        setRegister rd (fromIntegral oimm20 + pc)
+        setRegister rd (fromImm oimm20 + pc)
     | Jal rd jimm20 =>
         pc <- getPC;
-        let newPC := pc + (fromIntegral jimm20) in
+        let newPC := pc + (fromImm jimm20) in
         if (rem newPC four /= zero)
           then raiseException zero zero
           else (
-            setRegister rd (fromIntegral pc + four);;
+            setRegister rd (pc + four);;
             setPC newPC)
     | Jalr rd rs1 oimm12 =>
         x <- getRegister rs1;
         pc <- getPC;
-        let newPC := x + fromIntegral oimm12 in
+        let newPC := x + fromImm oimm12 in
         if (rem newPC four /= zero)
           then raiseException zero zero
           else (
-            setRegister rd (fromIntegral pc + four);;
+            setRegister rd (pc + four);;
             setPC newPC)
     | Beq rs1 rs2 sbimm12 =>
         x <- getRegister rs1;
         y <- getRegister rs2;
         pc <- getPC;
         when (x == y) (
-          let newPC := (pc + fromIntegral sbimm12) in
+          let newPC := (pc + fromImm sbimm12) in
           if (rem newPC four /= zero)
             then raiseException zero zero
             else setPC newPC)
@@ -91,7 +63,7 @@ Section Riscv.
         y <- getRegister rs2;
         pc <- getPC;
         when (x /= y) (
-          let addr := (pc + fromIntegral sbimm12) in
+          let addr := (pc + fromImm sbimm12) in
           if (rem addr four /= zero)
             then raiseException zero zero
             else setPC addr)
@@ -100,7 +72,7 @@ Section Riscv.
         y <- getRegister rs2;
         pc <- getPC;
         when (x < y) (
-          let addr := (pc + fromIntegral sbimm12) in
+          let addr := (pc + fromImm sbimm12) in
           if (rem addr four /= zero)
             then raiseException zero zero
             else setPC addr)
@@ -109,7 +81,7 @@ Section Riscv.
         y <- getRegister rs2;
         pc <- getPC;
         when (x >= y) (
-          let addr := (pc + fromIntegral sbimm12) in
+          let addr := (pc + fromImm sbimm12) in
           if (rem addr four /= zero)
             then raiseException zero zero
             else setPC addr)
@@ -118,7 +90,7 @@ Section Riscv.
         y <- getRegister rs2;
         pc <- getPC;
         when ((ltu x y)) (
-          let addr := (pc + fromIntegral sbimm12) in
+          let addr := (pc + fromImm sbimm12) in
           if (rem addr four /= zero)
             then raiseException zero zero
             else setPC addr)
@@ -127,85 +99,85 @@ Section Riscv.
         y <- getRegister rs2;
         pc <- getPC;
         when (negb (ltu x y)) (
-          let addr := (pc + fromIntegral sbimm12) in
+          let addr := (pc + fromImm sbimm12) in
           if (rem addr four /= zero)
             then raiseException zero zero
             else setPC addr)
     | Lb rd rs1 oimm12 =>
         a <- getRegister rs1;
-        withTranslation Load one (a + fromIntegral oimm12)
+        withTranslation Load one (a + fromImm oimm12)
           (fun addr => 
               x <- loadByte addr;
-              setRegister rd x)
+              setRegister rd (int8ToReg x))
     | Lh rd rs1 oimm12 =>
         a <- getRegister rs1;
-        withTranslation Load two (a + fromIntegral oimm12)
+        withTranslation Load two (a + fromImm oimm12)
           (fun addr => 
               x <- loadHalf addr;
-              setRegister rd x)
+              setRegister rd (int16ToReg x))
     | Lw rd rs1 oimm12 =>
         a <- getRegister rs1;
-        withTranslation Load four (a + fromIntegral oimm12)
+        withTranslation Load four (a + fromImm oimm12)
           (fun addr => 
               x <- loadWord addr;
-              setRegister rd x)
+              setRegister rd (int32ToReg x))
     | Lbu rd rs1 oimm12 =>
         a <- getRegister rs1;
-        withTranslation Load one (a + fromIntegral oimm12)
+        withTranslation Load one (a + fromImm oimm12)
           (fun addr => 
               x <- loadByte addr;
-              setRegister rd (unsigned x))
+              setRegister rd (uInt8ToReg x))
     | Lhu rd rs1 oimm12 =>
         a <- getRegister rs1;
-        withTranslation Load two (a + fromIntegral oimm12)
+        withTranslation Load two (a + fromImm oimm12)
           (fun addr => 
               x <- loadHalf addr;
-              setRegister rd (unsigned x))
+              setRegister rd (uInt16ToReg x))
     | Sb rs1 rs2 simm12 =>
         a <- getRegister rs1;
-        withTranslation Store one (a + fromIntegral simm12)
+        withTranslation Store one (a + fromImm simm12)
           (fun addr => 
               x <- getRegister rs2;
-              storeByte addr (fromIntegral x))
+              storeByte addr (regToInt8 x))
     | Sh rs1 rs2 simm12 =>
         a <- getRegister rs1;
-        withTranslation Store two (a + fromIntegral simm12)
+        withTranslation Store two (a + fromImm simm12)
           (fun addr => 
               x <- getRegister rs2;
-              storeHalf addr (fromIntegral x))
+              storeHalf addr (regToInt16 x))
     | Sw rs1 rs2 simm12 =>
         a <- getRegister rs1;
-        withTranslation Store four (a + fromIntegral simm12)
+        withTranslation Store four (a + fromImm simm12)
           (fun addr => 
               x <- getRegister rs2;
-              storeWord addr (fromIntegral x))
+              storeWord addr (regToInt32 x))
     | Addi rd rs1 imm12 =>
         x <- getRegister rs1;
-        setRegister rd (x + fromIntegral imm12)
+        setRegister rd (x + fromImm imm12)
     | Slti rd rs1 imm12 =>
         x <- getRegister rs1;
-        setRegister rd (if x < (fromIntegral imm12) then one else zero)
+        setRegister rd (if x < (fromImm imm12) then one else zero)
     | Sltiu rd rs1 imm12 =>
         x <- getRegister rs1;
-        setRegister rd (if (ltu x imm12) then one else zero)
+        setRegister rd (if (ltu x (fromImm imm12)) then one else zero)
     | Xori rd rs1 imm12 =>
         x <- getRegister rs1;
-        setRegister rd (xor x (fromIntegral imm12))
+        setRegister rd (xor x (fromImm imm12))
     | Ori rd rs1 imm12 =>
         x <- getRegister rs1;
-        setRegister rd (x <|> (fromIntegral imm12))
+        setRegister rd (x <|> (fromImm imm12))
     | Andi rd rs1 imm12 =>
         x <- getRegister rs1;
-        setRegister rd (x <&> (fromIntegral imm12))
+        setRegister rd (x <&> (fromImm imm12))
     | Slli rd rs1 shamt6 =>
         x <- getRegister rs1;
-        setRegister rd (slli x shamt6)
+        setRegister rd (sll x (regToShamt (fromImm shamt6 : t)))
     | Srli rd rs1 shamt6 =>
         x <- getRegister rs1;
-        setRegister rd (srli x shamt6)
+        setRegister rd (srl x (regToShamt (fromImm shamt6 : t)))
     | Srai rd rs1 shamt6 =>
         x <- getRegister rs1;
-        setRegister rd (srai x shamt6)
+        setRegister rd (sra x (regToShamt (fromImm shamt6 : t)))
     | Add rd rs1 rs2 =>
         x <- getRegister rs1;
         y <- getRegister rs2;
@@ -217,7 +189,7 @@ Section Riscv.
     | Sll rd rs1 rs2 =>
         x <- getRegister rs1;
         y <- getRegister rs2;
-        setRegister rd (sll x y)
+        setRegister rd (sll x (regToShamt y))
     | Slt rd rs1 rs2 =>
         x <- getRegister rs1;
         y <- getRegister rs2;
@@ -237,11 +209,11 @@ Section Riscv.
     | Srl rd rs1 rs2 =>
         x <- getRegister rs1;
         y <- getRegister rs2;
-        setRegister rd (srl x y)
+        setRegister rd (srl x (regToShamt y))
     | Sra rd rs1 rs2 =>
         x <- getRegister rs1;
         y <- getRegister rs2;
-        setRegister rd (sra x y)
+        setRegister rd (sra x (regToShamt y))
     | And rd rs1 rs2 =>
         x <- getRegister rs1;
         y <- getRegister rs2;
