src/NoVirtualMemory.v
@@ -1,3 +1,4 @@
+Require Import riscv.Utility.
 Require Import riscv.Program.
 Require Import riscv.util.Monad.
 Require Import riscv.util.NameWithEq.
@@ -8,7 +9,7 @@ Local Open Scope alu_scope.
 
 (* in a system with virtual memory, this would also do the translation, but in our
    case, we only verify the alignment *)
-Definition withTranslation{N: NameWithEq}{t u: Set}{A: Alu t u}{M: Type -> Type}
+Definition withTranslation{N: NameWithEq}{t: Set}{MW: MachineWidth t}{M: Type -> Type}
   {MM: Monad M}{RVS: RiscvState M}
   (accessType: AccessType)(alignment: t)(addr: t)(memFunc: t -> M unit): M unit :=
   if rem addr alignment /= zero
